Pass through a C AST for to_string

src/Experiments/SimplyTypedArithmetic.v
@@ -33,7 +33,7 @@ Require Import Crypto.Util.Tactics.SpecializeBy.
 Require Import Crypto.Util.Tactics.SplitInContext.
 Require Import Crypto.Util.Tactics.SubstEvars.
 Require Import Crypto.Util.Strings.Decimal.
-Require Import Crypto.Util.Strings.Hex.
+Require Import Crypto.Util.Strings.HexString.
 Require Import Crypto.Util.Notations.
 Require Import Crypto.Util.ZUtil.Definitions.
 Require Import Crypto.Util.ZUtil.CC Crypto.Util.ZUtil.Rshi.
@@ -6068,65 +6068,125 @@ Module Compilers.
     Definition Reassociate (max_const_val : Z) {t} (e : Expr t) : Expr t
       := fun var => reassociate max_const_val (e _).
   End ReassociateSmallConstants.
-<<<<<<< d97e060a3f8de0b83db89aa6c25eb4157045c275
-||||||| merged common ancestors
-=======
-      Module ToString.
-        Import Coq.Strings.String.
-        Import Coq.Strings.Ascii.
-        Local Open Scope string_scope.
 
-        Module Z.
-          Definition to_hex_string (v : Z) : string
-            := match v with
-               | Zpos p => hex_string_of_pos p
-               | Z0 => "0x0"
-               | Zneg p => String "-" (hex_string_of_pos p)
-               end.
+  Module ToString.
+    Import Coq.Strings.String.
+    Import Coq.Strings.Ascii.
+    Local Open Scope string_scope.
 
-          Definition to_decimal_string (v : Z) : string
-            := match v with
-               | Zpos p => decimal_string_of_pos p
-               | Z0 => "0"
-               | Zneg p => String "-" (decimal_string_of_pos p)
-               end.
-        End Z.
+    Module Z.
+      Definition to_hex_string (v : Z) : string
+        := HexString.of_Z v.
 
-        Module primitive.
-          Definition to_UL_postfix (t : type.primitive) : string
-            := match t with
-               | type.unit => ""
-               | type.Z => ""
-               | type.ZBounded lower upper
-                 => let u := (if lower >=? 0 then "U" else "") in
-                    let sz := Z.log2_up (Z.max (Z.abs upper + 1) (Z.abs lower)) in
-                    if sz <=? 32
-                    then ""
-                    else if sz <=? 64
-                         then u ++ "L"
-                         else if sz <=? 128
-                              then u ++ "LL"
-                              else " /* " ++ Z.to_hex_string lower ++ " <= val <= " ++ Z.to_hex_string upper ++ " */"
-               end.
+      Definition to_decimal_string (v : Z) : string
+        := match v with
+           | Zpos p => decimal_string_of_pos p
+           | Z0 => "0"
+           | Zneg p => String "-" (decimal_string_of_pos p)
+           end.
+    End Z.
 
-          Definition to_string {t} (v : type.primitive.interp t) : string
-            := match t return type.primitive.interp t -> string with
-               | type.unit => fun 'tt => "#error tt;"
-               | type.Z => fun v => Z.to_hex_string v ++ "ℤ"
-               | type.ZBounded lower upper
-                 => fun v
-                    => (Z.to_hex_string (type.value v))
-                         ++ to_UL_postfix t
-               end v.
-        End primitive.
+    Module C.
+      Module type.
+        Inductive primitive := Z | Zptr.
+        Inductive type := type_primitive (t : primitive) | prod (A B : type) | unit.
+        Module Export Notations.
+          Global Coercion type_primitive : primitive >-> type.
+          Delimit Scope Ctype_scope with Ctype.
+          Bind Scope Ctype_scope with type.
+          Notation "()" := unit : Ctype_scope.
+          Notation "A * B" := (prod A B) : Ctype_scope.
+          Notation type := type.
+        End Notations.
+      End type.
+      Import type.Notations.
 
+      Section ident.
+        Import type.
+        Inductive ident : type -> type -> Set :=
+        | literal (v : BinInt.Z) : ident unit Z
+        | List_nth (n : Datatypes.nat) : ident Zptr Z
+        | Addr : ident Z Zptr
+        | Dereference : ident Zptr Z
+        | Z_shiftr (offset : BinInt.Z) : ident Z Z
+        | Z_shiftl (offset : BinInt.Z) : ident Z Z
+        | Z_land (mask : BinInt.Z) : ident Z Z
+        | Z_add : ident (Z * Z) Z
+        | Z_mul : ident (Z * Z) Z
+        | Z_sub : ident (Z * Z) Z
+        | Z_opp : ident Z Z
+        | Z_mul_split (s:BinInt.Z) : ident (Z * Z * Zptr) Z
+        | Z_add_get_carry (s:BinInt.Z) : ident (Z * Z * Zptr) Z
+        | Z_add_with_get_carry (s:BinInt.Z) : ident (Z * Z * Z * Zptr) Z
+        | Z_sub_get_borrow (s:BinInt.Z) : ident (Z * Z * Zptr) Z
+        | Z_zselect : ident (Z * Z * Z) Z
+        | Z_add_modulo : ident (Z * Z * Z) Z
+        | Z_static_cast (range : zrange) : ident Z Z
+        .
+      End ident.
+
+      Inductive arith_expr : type -> Set :=
+      | AppIdent {s d} (idc : ident s d) (arg : arith_expr s) : arith_expr d
+      | Var (t : type.primitive) (v : string) : arith_expr t
+      | Pair {A B} (a : arith_expr A)( b : arith_expr B) : arith_expr (A * B)
+      | TT : arith_expr type.unit.
+
+      Inductive expr :=
+      | Seq (e1 : expr) (e2 : expr) : expr
+      | Assign (declare : bool) (t : type.primitive) (sz : option zrange) (name : string) (val : arith_expr t)
+      | AssignZPtr (name : string) (sz : option zrange) (val : arith_expr type.Z)
+      | DeclareVar (t : type.primitive) (sz : option zrange) (name : string)
+      | AssignNth (name : string) (n : nat) (val : arith_expr type.Z).
+
+      Fixpoint splice_seq (e1 e2 : expr) {struct e1} : expr
+        := match e1, e2 with
+           | Seq e0 e1, _
+             => splice_seq e0 (splice_seq e1 e2)
+           | _, _ => Seq e1 e2
+           end.
+
+      Module Export Notations.
+        Export type.Notations.
+        Delimit Scope Cexpr_scope with Cexpr.
+        Bind Scope Cexpr_scope with expr.
+        Bind Scope Cexpr_scope with arith_expr.
+        Infix "@@" := AppIdent : Cexpr_scope.
+        Notation "( x , y , .. , z )" := (Pair .. (Pair x%Cexpr y%Cexpr) .. z%Cexpr) : Cexpr_scope.
+        Notation "( )" := TT : Cexpr_scope.
+        Notation "()" := TT : Cexpr_scope.
+      End Notations.
+
+      Module primitive.
+        Definition small_enough (v : Z) : bool
+          := Z.log2_up (Z.abs v + 1) <=? 128.
+        Definition to_UL_postfix (r : zrange) : string
+          := let lower := lower r in
+             let upper := upper r in
+             let u := (if lower >=? 0 then "U" else "") in
+             let sz := Z.log2_up (Z.max (Z.abs upper + 1) (Z.abs lower)) in
+             if sz <=? 32
+             then ""
+             else if sz <=? 64
+                  then u ++ "L"
+                  else if sz <=? 128
+                       then u ++ "LL"
+                       else " /* " ++ Z.to_hex_string lower ++ " <= val <= " ++ Z.to_hex_string upper ++ " */".
+
+        Definition to_string {t : type.primitive} (v : BinInt.Z) : string
+          := match t with
+             | type.Z => Z.to_hex_string v ++ (if small_enough v
+                                               then to_UL_postfix r[v~>v]
+                                               else "ℤ")
+             | type.Zptr => "#error ""literal address " ++ Z.to_hex_string v ++ """;"
+             end.
+      End primitive.
+
+      Module String.
         Module type.
           Module primitive.
-            Definition to_string (t : type.primitive) : string
-              := match t with
-                 | type.unit => "unit"
-                 | type.Z => "ℤ"
-                 | type.ZBounded lower upper
+            Definition to_string (t : type.primitive) (r : option zrange) : string
+              := match r with
+                 | Some r[ lower ~> upper ]%zrange
                    => let lg2u := Z.log2_up (upper + 1) in
                       let default := "ℤ[" ++ Z.to_hex_string lower ++ "," ++ Z.to_hex_string upper ++ "]" in
                       if (2^lg2u - 1 =? upper) && (lower =? 0)
@@ -6134,495 +6194,833 @@ Module Compilers.
                       else if (-2^lg2u =? lower) && (2^lg2u - 1 =? upper)
                            then "int" ++ Z.to_decimal_string lg2u ++ "_t"
                            else default
-                 end.
+                 | None
+                   => "ℤ"
+                 end ++ match t with
+                        | type.Zptr => "*"
+                        | type.Z => ""
+                        end.
+            Definition to_string_relaxed (t : type.primitive) (r : option zrange) : string
+              := match r with
+                 | Some r[ lower ~> upper ]%zrange
+                   => let lg2u := Z.log2_up (upper + 1) in
+                      let lg2lg2u := Z.log2_up lg2u in
+                      let lg2u := 2^lg2lg2u in
+                      let default := "ℤ[" ++ Z.to_hex_string lower ++ "," ++ Z.to_hex_string upper ++ "]" in
+                      if (0 <=? lower) && (upper <=? 2^lg2u - 1)
+                      then "uint" ++ Z.to_decimal_string lg2u ++ "_t"
+                      else if (-2^lg2u <=? lower) && (upper <=? 2^lg2u - 1)
+                           then "int" ++ Z.to_decimal_string lg2u ++ "_t"
+                           else default
+                 | None
+                   => "ℤ"
+                 end ++ match t with
+                        | type.Zptr => "*"
+                        | type.Z => ""
+                        end.
           End primitive.
-
-          Fixpoint to_string (t : type) : string
-            := match t with
-               | type.type_primitive x => primitive.to_string x
-               | type.prod A B => to_string A ++ " * " ++ to_string B
-               | type.list A => primitive.to_string A ++ "*"
-               end.
-
-          Fixpoint string_interp (t : type) : Set
-            := match t with
-               | type.type_primitive x => string
-               | type.prod A B => string_interp A * string_interp B
-               | type.list A => list string + string
-               end.
         End type.
+      End String.
 
-        Module ident.
-          Definition infix_to_string (op : string) (long_op : string)
-                     (T1 T2 Tout : type.primitive) (x y : string)
-          : string
-            := match T1, T2, Tout with
-               | type.unit, _, _
-               | _, type.unit, _
-               | _, _, type.unit
-                 => "(" ++ x ++ " " ++ op ++ "ᵤₙᵢₜ " ++ y ++ ")"
-               | type.Z, _, _
-               | _, type.Z, _
-               | _, _, type.Z
-                 => "(" ++ x ++ " " ++ op ++ "ℤ " ++ y ++ ")"
-               | T1, T2, Tout
-                 => if type.primitive_beq T1 Tout && type.primitive_beq T2 Tout
-                    then "(" ++ x ++ " " ++ op ++ " " ++ y ++ ")"
-                    else if ((type.primitive_beq Tout (type.primitive.max (type.primitive.max T1 T2) Tout))
-                               && (type.primitive_beq T1 Tout || type.primitive_beq T2 Tout))
-                         then (* don't need to cast if the output is the largest size and either of the inputs is the output size *)
-                           "(" ++ x ++ " " ++ op ++ " " ++ y ++ ")"
-                         else if type.primitive_beq Tout (type.primitive.max (type.primitive.max T1 T2) Tout)
-                              then
-                                "((" ++ type.to_string Tout ++ ")" ++ x ++ " " ++ op ++ " " ++ y ++ ")"
-                              else
-                                long_op ++ "_" ++ type.to_string T1 ++ "_" ++ type.to_string T2 ++ "_" ++ type.to_string Tout ++ "(" ++ x ++ ", " ++ y ++ ")"
-               end.
-          Definition mul_to_string (T1 T2 Tout : type.primitive) (x y : string)
-            : string
-            := infix_to_string "*" "mul" T1 T2 Tout x y.
-          Definition add_to_string (T1 T2 Tout : type.primitive) (x y : string)
-            : string
-            := infix_to_string "+" "add" T1 T2 Tout x y.
+      Fixpoint var_data (t : Compilers.type.type) : Set
+        := match t with
+           | Compilers.type.unit
+             => unit
+           | type.nat
+           | type.bool
+           | type.arrow _ _
+             => Empty_set
+           | Compilers.type.Z => string * option zrange
+           | Compilers.type.prod A B => var_data A * var_data B
+           | type.list A => string * option zrange * nat
+           end.
+
+      Fixpoint arith_expr_for (t : Compilers.type.type) : Set
+        := match t with
+           | Compilers.type.Z
+             => arith_expr type.Z * option zrange
+           | Compilers.type.prod A B
+             => arith_expr_for A * arith_expr_for B
+           | type.list A => list (arith_expr_for A)
+           | Compilers.type.unit
+             => Datatypes.unit
+           | type.nat
+           | type.bool
+           | type.arrow _ _
+             => Empty_set
+           end.
+
+      (** Quoting http://en.cppreference.com/w/c/language/conversion:
+
+          ** Integer promotions
+
+          Integer promotion is the implicit conversion of a value of
+          any integer type with rank less or equal to rank of int or
+          of a bit field of type _Bool, int, signed int, unsigned int,
+          to the value of type int or unsigned int
+
+          If int can represent the entire range of values of the
+          original type (or the range of values of the original bit
+          field), the value is converted to type int. Otherwise the
+          value is converted to unsigned int. *)
+      (** We assume a 32-bit [int] type *)
+      Definition integer_promote_range (r : zrange) : zrange
+        := (let '(l, u) := (lower r, upper r) in
+            if (0 <=? l) && (u <=? 2^32-1)
+            then r[0 ~> 2^32-1]
+            else if (-2^31 <=? l) && (u <=? 2^31-1)
+                 then r[-2^31 ~> 2^31-1]
+                 else r)%Z%bool%zrange.
+
+      (** Quoting http://en.cppreference.com/w/c/language/conversion:
+
+          First of all, both operands undergo integer promotions (see
+          below). Then
+
+          - If the types after promotion are the same, that type is
+            the common type
+
+          - Otherwise, if both operands after promotion have the same
+            signedness (both signed or both unsigned), the operand
+            with the lesser conversion rank (see below) is implicitly
+            converted to the type of the operand with the greater
+            conversion rank
+
+          - Otherwise, the signedness is different: If the operand
+            with the unsigned type has conversion rank greater or
+            equal than the rank of the type of the signed operand,
+            then the operand with the signed type is implicitly
+            converted to the unsigned type
+
+          - Otherwise, the signedness is different and the signed
+            operand's rank is greater than unsigned operand's rank. In
+            this case, if the signed type can represent all values of
+            the unsigned type, then the operand with the unsigned type
+            is implicitly converted to the type of the signed operand.
+
+          - Otherwise, both operands undergo implicit conversion to
+            the unsigned type counterpart of the signed operand's
+            type. *)
+            (** Quoting http://en.cppreference.com/w/c/language/conversion:
+
+          rank above is a property of every integer type and is
+          defined as follows:
+
+          1) the ranks of all signed integer types are different and
+             increase with their precision: rank of signed char < rank
+             of short < rank of int < rank of long int < rank of long
+             long int
+
+          2) the ranks of all signed integer types equal the ranks of
+             the corresponding unsigned integer types
+
+          3) the rank of any standard integer type is greater than the
+             rank of any extended integer type of the same size (that
+             is, rank of __int64 < rank of long long int, but rank of
+             long long < rank of __int128 due to the rule (1))
+
+          4) rank of char equals rank of signed char and rank of
+             unsigned char
+
+          5) the rank of _Bool is less than the rank of any other
+             standard integer type
+
+          6) the rank of any enumerated type equals the rank of its
+             compatible integer type
+
+          7) ranking is transitive: if rank of T1 < rank of T2 and
+             rank of T2 < rank of T3 then rank of T1 < rank of T3
+
+          8) any aspects of relative ranking of extended integer types
+             not covered above are implementation defined *)
+      (** We define the rank to be the bitwidth, which satisfies (1),
+          (2), (4), (5), and (7).  Points (3) and (6) do not apply. *)
+      Definition rank (r : zrange) : BinInt.Z
+        := Z.log2_up (Z.abs (upper r - lower r) + 1).
+      Definition unsigned_counterpart_of (r : zrange) : zrange
+        := let '(l, u) := (lower r, upper r) in
+           if 0 <=? l then
+             r
+           else let sz := Z.log2_up (Z.abs (u - l) + 1) in
+                r[ 0 ~> 2^sz-1 ].
+      Definition IMPOSSIBLE {T} (v : T) : T. exact v. Qed.
+      Definition common_type (r1 r2 : zrange) : zrange
+        := (let r1 := integer_promote_range r1 in
+            let r2 := integer_promote_range r2 in
+            let '(l1, u1) := (lower r1, upper r1) in
+            let '(l2, u2) := (lower r2, upper r2) in
+            if (l1 =? l2) && (u1 =? u2) then
+              r1
+            else if ((0 <=? l1) && (0 <=? l2))
+                    || ((l1 <? 0) && (l2 <? 0)) then
+                   r[ Z.min l1 l2  ~>  Z.max u1 u2 ]
+            else if (0 <=? l1) && (l2 <? 0) && (rank r1 >=? rank r2) then
+                   r1
+            else if (0 <=? l2) && (l1 <? 0) && (rank r2 >=? rank r1) then
+                   r2
+            else if (l1 <? 0) && (0 <=? l2) && (rank r1 >? rank r2) then
+                   r1
+            else if (l2 <? 0) && (0 <=? l1) && (rank r2 >? rank r1) then
+                   r2
+            else if (l1 <? 0) && (0 <=? l2) then
+                   unsigned_counterpart_of r1
+            else if (l2 <? 0) && (0 <=? l1) then
+                   unsigned_counterpart_of r2
+            else IMPOSSIBLE ZRange.union r1 r2).
+
+      Fixpoint cast_down_if_needed {t}
+        : ZRange.type.option.interp t -> arith_expr_for t -> arith_expr_for t
+        := match t return ZRange.type.option.interp t -> arith_expr_for t -> arith_expr_for t with
+           | Compilers.type.Z
+             => fun r1 '(e, r)
+                => match r1, r with
+                   | None, _ => (e, r)
+                   | Some r1, Some r
+                     => if is_tighter_than_bool r r1
+                        then (e, Some r)
+                        else (Z_static_cast r1 @@ e, Some r1)%core%Cexpr
+                   | Some r1, None
+                     => (Z_static_cast r1 @@ e, Some r1)%core%Cexpr
+                   end
+           | Compilers.type.type_primitive _ => fun _ x => x
+           | Compilers.type.prod A B
+             => fun '(r1, r2) '(e1, e2) => (@cast_down_if_needed A r1 e1,
+                                            @cast_down_if_needed B r2 e2)
+           | type.arrow s d => fun _ x => x
+           | type.list A
+             => fun r1 ls
+                => match r1 with
+                   | Some r1 => List.map (fun '(r, e) => @cast_down_if_needed A r e)
+                                         (List.combine r1 ls)
+                   | None => ls
+                   end
+           end.
+
+      Fixpoint cast_up_if_needed {t}
+        : ZRange.type.option.interp t -> arith_expr_for t -> arith_expr_for t
+        := match t return ZRange.type.option.interp t -> arith_expr_for t -> arith_expr_for t with
+           | Compilers.type.Z
+             => fun r1 '(e, r)
+                => match r1, r with
+                   | None, _ | _, None => (e, r)
+                   | Some r1, Some r
+                     => if is_tighter_than_bool r1 r
+                        then (e, Some r)
+                        else (Z_static_cast r1 @@ e, Some r1)%core%Cexpr
+                   end
+           | Compilers.type.type_primitive _ => fun _ x => x
+           | Compilers.type.prod A B
+             => fun '(r1, r2) '(e1, e2) => (@cast_up_if_needed A r1 e1,
+                                            @cast_up_if_needed B r2 e2)
+           | type.arrow s d => fun _ x => x
+           | type.list A
+             => fun r1 ls
+                => match r1 with
+                   | Some r1 => List.map (fun '(r, e) => @cast_up_if_needed A r e)
+                                         (List.combine r1 ls)
+                   | None => ls
+                   end
+           end.
+
+      Definition cast_bigger_up_if_needed
+                 (rout : option zrange)
+                 (args : arith_expr_for (Compilers.type.Z * Compilers.type.Z))
+        : arith_expr_for (Compilers.type.Z * Compilers.type.Z)
+        := match rout with
+           | None => args
+           | Some rout
+             => let '((e1, r1), (e2, r2)) := args in
+                match r1, r2 with
+                | None, _ | _, None => args
+                | Some r1', Some r2'
+                  => if is_tighter_than_bool r2' r1'
+                     then (cast_up_if_needed (t:=Compilers.type.Z) (Some rout) (e1, r1), (e2, r2))
+                     else ((e1, r1), cast_up_if_needed (t:=Compilers.type.Z) (Some rout) (e2, r2))
+                end
+           end.
+
+      Definition arith_bin_arith_expr_of_PHOAS_ident
+                 (s:=(Compilers.type.Z * Compilers.type.Z)%ctype)
+                 (d:=Compilers.type.Z)
+                 (idc : ident (type.Z * type.Z) type.Z)
+        : ZRange.type.option.interp d -> arith_expr_for s -> option (arith_expr_for d)
+        := fun rout '((e1, r1), (e2, r2))
+           => let r1 := option_map integer_promote_range r1 in
+              let r2 := option_map integer_promote_range r2 in
+              let ct := (r1 <- r1; r2 <- r2; Some (common_type r1 r2))%option in
+              let '((e1, r1), (e2, r2))
+                  := cast_bigger_up_if_needed rout ((e1, r1), (e2, r2)) in
+              Some (cast_down_if_needed rout ((idc @@ (e1, e2))%Cexpr, ct)).
+
+      Definition arith_expr_of_PHOAS_ident
+                 {s d}
+                 (idc : default.ident.ident s d)
+        : ZRange.type.option.interp d -> arith_expr_for s -> option (arith_expr_for d)
+        := match idc in default.ident.ident s d return ZRange.type.option.interp d -> arith_expr_for s -> option (arith_expr_for d) with
+           | ident.primitive Compilers.type.Z v
+             => fun r _ => Some (cast_down_if_needed
+                                   r
+                                   (literal v @@ TT, Some r[v~>v]%zrange))
+           | ident.nil t
+             => fun _ _ => Some nil
+           | ident.cons t
+             => fun r '(x, xs) => Some (cast_down_if_needed r (cons x xs))
+           | ident.fst A B => fun r xy => Some (cast_down_if_needed r (@fst _ _ xy))
+           | ident.snd A B => fun r xy => Some (cast_down_if_needed r (@snd _ _ xy))
+           | ident.List_nth_default_concrete Compilers.type.Z d n
+             => fun r ls
+                => List.nth_default None (List.map (fun x => Some (cast_down_if_needed r x)) ls) n
+           | ident.Z_shiftr offset
+             => fun rout '(e, r)
+                => let rin := option_map integer_promote_range r in
+                   Some (cast_down_if_needed rout (Z_shiftr offset @@ e, rin))
+           | ident.Z_shiftl offset
+             => fun rout '(e, r)
+                => let rin := option_map integer_promote_range r in
+                   let '(e', rin') := cast_up_if_needed rout (e, rin) in
+                   Some (cast_down_if_needed rout (Z_shiftr offset @@ e', rin'))
+           | ident.Z_land mask
+             => fun rout '(e, r)
+                => Some (cast_down_if_needed
+                           rout
+                           (Z_land mask @@ e,
+                            option_map integer_promote_range r))
+           | ident.Z_add => arith_bin_arith_expr_of_PHOAS_ident Z_add
+           | ident.Z_mul => arith_bin_arith_expr_of_PHOAS_ident Z_mul
+           | ident.Z_sub => arith_bin_arith_expr_of_PHOAS_ident Z_sub
+           | ident.Z_zselect
+             => fun rout '((econd, _), (e1, r1), (e2, r2))
+                => let r1 := option_map integer_promote_range r1 in
+                   let r2 := option_map integer_promote_range r2 in
+                   let ct := (r1 <- r1; r2 <- r2; Some (common_type r1 r2))%option in
+                   let '((e1, r1), (e2, r2))
+                       := cast_bigger_up_if_needed rout ((e1, r1), (e2, r2)) in
+                   Some (cast_down_if_needed rout ((Z_zselect @@ (econd, e1, e2))%Cexpr, ct))
+           | ident.primitive _ _
+           | ident.Let_In _ _
+           | ident.Nat_succ
+           | ident.Nat_add
+           | ident.Nat_sub
+           | ident.Nat_mul
+           | ident.Nat_max
+           | ident.bool_rect _
+           | ident.nat_rect _
+           | ident.pred
+           | ident.list_rect _ _
+           | ident.List_nth_default _
+           | ident.List_nth_default_concrete _ _ _
+           | ident.Z_pow
+           | ident.Z_div
+           | ident.Z_modulo
+           | ident.Z_eqb
+           | ident.Z_leb
+           | ident.Z_of_nat
+           | ident.Z_opp
+           | ident.Z_mul_split
+           | ident.Z_mul_split_concrete _
+           | ident.Z_add_get_carry
+           | ident.Z_add_get_carry_concrete _
+           | ident.Z_add_with_get_carry
+           | ident.Z_add_with_get_carry_concrete _
+           | ident.Z_sub_get_borrow
+           | ident.Z_sub_get_borrow_concrete _
+           | ident.Z_cast _
+           | ident.Z_cast2 _
+           | ident.Z_add_modulo
+             => fun _ _ => None
+           end%core%Cexpr.
+
+      Fixpoint arith_expr_of_PHOAS_Var
+               {t}
+        : var_data t -> ZRange.type.option.interp t -> option (arith_expr_for t)
+        := match t with
+           | Compilers.type.Z
+             => fun '(n, r) r' => Some (cast_down_if_needed r' (Var type.Z n, r))
+           | Compilers.type.prod A B
+             => fun '(da, db) '(ra, rb)
+                => (ea <- @arith_expr_of_PHOAS_Var A da ra;
+                      eb <- @arith_expr_of_PHOAS_Var B db rb;
+                      Some (ea, eb))%option
+           | type.list Compilers.type.Z
+             => fun '(n, r, len) r'
+                => Some (List.map
+                           (fun i => (List_nth i @@ Var type.Zptr n, r))%core%Cexpr
+                           (List.seq 0 len))
+           | type.list _
+           | Compilers.type.type_primitive _
+           | type.arrow _ _
+             => fun _ _ => None
+           end.
+
+      Fixpoint arith_expr_of_PHOAS
+               {t}
+               (e : @Compilers.Uncurried.expr.default.Notations.expr var_data t)
+        : ZRange.type.option.interp t -> option (arith_expr_for t)
+        := match e in expr.expr t return ZRange.type.option.interp t -> option (arith_expr_for t) with
+           | expr.Var t v
+             => @arith_expr_of_PHOAS_Var t v
+           | expr.TT
+             => fun _ => Some tt
+           | expr.Pair A B a b
+             => fun '(ra, rb)
+                => (a' <- @arith_expr_of_PHOAS A a ra;
+                      b' <- @arith_expr_of_PHOAS B b rb;
+                      Some (a', b'))%option
+           | Abs _ _ _
+           | App _ _ _ _
+             => fun _ => None
+           | expr.AppIdent s d idc args
+             => fun rout
+                => let of_args _ rin := @arith_expr_of_PHOAS s args rin in
+                   let default _
+                       := (args' <- of_args tt ZRange.type.option.None;
+                             arith_expr_of_PHOAS_ident idc rout args') in
+                   match idc in default.ident.ident s d
+                         return (unit -> option (arith_expr_for d))
+                                -> (unit -> ZRange.type.option.interp s -> option (arith_expr_for s))
+                                -> ZRange.type.option.interp d
+                                -> option (arith_expr_for d)
+                   with
+                   | ident.Z_cast range
+                     => fun _ of_args rout
+                        => (args' <- of_args tt (Some range);
+                              Some (cast_down_if_needed rout args'))
+                   | ident.Z_cast2 (r1, r2)
+                     => fun _ of_args rout
+                        => (args' <- of_args tt (Some r1, Some r2);
+                              Some (cast_down_if_needed rout args'))
+                   | ident.nil _
+                     => fun _ _ _ => Some nil
+                   | ident.cons t
+                     => fun default of_args (rout : option (list (ZRange.type.option.interp t)))
+                        => match rout with
+                           | Some (cons r rs)
+                             => (args' <- of_args tt (r, Some rs);
+                                   arith_expr_of_PHOAS_ident ident.cons rout args')
+                           | Some nil => default tt
+                           | None => default tt
+                           end
+                   | _ => fun default _ _ => default tt
+                   end default of_args rout
+           end%option.
+
+      Fixpoint make_return_assignment_of_arith {t}
+        : var_data t
+          -> @Compilers.Uncurried.expr.default.Notations.expr var_data t
+          -> option expr
+        := match t return var_data t -> default.Notations.expr t -> _ with
+           | Compilers.type.Z
+             => fun '(n, r) e
+                => (rhs <- arith_expr_of_PHOAS e r;
+                      let '(e, r) := rhs in
+                      Some (AssignZPtr n r e))
+           | Compilers.type.type_primitive _ => fun _ _ => None
+           | Compilers.type.prod A B
+             => fun '(rva, rvb) e
+                => match invert_Pair e with
+                   | Some (ea, eb)
+                     => (ea' <- @make_return_assignment_of_arith A rva ea;
+                           eb' <- @make_return_assignment_of_arith B rvb eb;
+                           Some (splice_seq ea' eb'))
+                   | None => None
+                   end
+           | type.arrow s d => fun _ _ => None
+           | type.list Compilers.type.Z
+             => fun '(n, r, len) e
+                => (ls <- arith_expr_of_PHOAS e (Some (List.repeat r len));
+                      List.fold_right
+                        (fun a b
+                         => match b with
+                            | Some b => Some (splice_seq a b)
+                            | None => Some a
+                            end)
+                        None
+                        (List.map
+                           (fun '(i, (e, _)) => AssignNth n i e)
+                           (List.combine (List.seq 0 len) ls)))
+           | type.list _ => fun _ _ => None
+           end%option.
+
+      Definition make_assign_2arg_1ref
+                 {t1 t2 d t3}
+                 (r1 r2 : option zrange)
+                 (x1 : @Compilers.Uncurried.expr.default.Notations.expr var_data t1)
+                 (x2 : @Compilers.Uncurried.expr.default.Notations.expr var_data t2)
+                 (idc : ident (type.Z * type.Z * type.Zptr) type.Z)
+                 (count : positive)
+                 (make_name : positive -> option string)
+                 (v : var_data t3)
+                 (e2 : var_data d -> var_data (Compilers.type.Z * Compilers.type.Z)%ctype -> option expr)
+        : option expr
+        := (v <- type.try_transport var_data _ d v;
+              x1 <- type.try_transport expr.expr _ Compilers.type.Z x1;
+              x2 <- type.try_transport expr.expr _ Compilers.type.Z x2;
+              let e2 := e2 v in
+              x1 <- arith_expr_of_PHOAS x1 None;
+              x2 <- arith_expr_of_PHOAS x2 None;
+              let '(x1, x1r) := x1 in
+              let '(x2, x2r) := x2 in
+              n1 <- make_name count;
+                n2 <- make_name (Pos.succ count);
+                e2 <- e2 ((n1, r1), (n2, r2));
+                Some (Seq
+                        (DeclareVar type.Z r2 n2)
+                        (Seq
+                           (Assign true type.Z r1 n1 (idc @@ (x1, x2, Addr @@ Var type.Z n2)))
+                           e2)))%option.
+
+      Definition make_assign_3arg_1ref
+                 {t1 t2 t3 d t4}
+                 (r1 r2 : option zrange)
+                 (x1 : @Compilers.Uncurried.expr.default.Notations.expr var_data t1)
+                 (x2 : @Compilers.Uncurried.expr.default.Notations.expr var_data t2)
+                 (x3 : @Compilers.Uncurried.expr.default.Notations.expr var_data t3)
+                 (idc : ident (type.Z * type.Z * type.Z * type.Zptr) type.Z)
+                 (count : positive)
+                 (make_name : positive -> option string)
+                 (v : var_data t4)
+                 (e2 : var_data d -> var_data (Compilers.type.Z * Compilers.type.Z)%ctype -> option expr)
+        : option expr
+        := (v <- type.try_transport var_data _ d v;
+              x1 <- type.try_transport expr.expr _ Compilers.type.Z x1;
+              x2 <- type.try_transport expr.expr _ Compilers.type.Z x2;
+              x3 <- type.try_transport expr.expr _ Compilers.type.Z x3;
+              let e2 := e2 v in
+              x1 <- arith_expr_of_PHOAS x1 None;
+              x2 <- arith_expr_of_PHOAS x2 None;
+              x3 <- arith_expr_of_PHOAS x3 None;
+              let '(x1, x1r) := x1 in
+              let '(x2, x2r) := x2 in
+              let '(x3, x3r) := x3 in
+              n1 <- make_name count;
+                n2 <- make_name (Pos.succ count);
+                e2 <- e2 ((n1, r1), (n2, r2));
+                Some (Seq
+                        (DeclareVar type.Z r2 n2)
+                        (Seq
+                           (Assign true type.Z r1 n1 (idc @@ (x1, x2, x3, Addr @@ Var type.Z n2)))
+                           e2)))%option.
 
 
-          Definition to_string {s d} (idc : ident s d) : type.string_interp s -> type.string_interp d
-            := match idc in ident s d return type.string_interp s -> type.string_interp d with
-               | ident.primitive t v => fun _ => primitive.to_string v
-               | ident.nil t => fun _ => inl nil
-               | ident.cons t
-                 => fun '(x, xs)
-                    => match xs with
-                       | inl xs => inl (x :: xs)
-                       | inr sxs => inl (x :: ("static_assert(false); /* variable list in cos: " ++ sxs ++ " */") :: nil)
-                       end
-               | ident.fst A B => @Datatypes.fst (type.string_interp A) (type.string_interp B)
-               | ident.snd A B => @Datatypes.snd (type.string_interp A) (type.string_interp B)
-               | ident.List_nth T n
-                 => fun ls
-                    => match ls with
-                       | inl ls => List.nth_default
-                                     ("((void*)0)[" ++ Z.to_decimal_string (Z.of_nat n) ++ "]")
-                                     ls n
-                       | inr sls => sls ++ "[" ++ Z.to_decimal_string (Z.of_nat n) ++ "]"
-                       end
-               | ident.mul T1 T2 Tout
-                 => fun '(x, y)
-                    => mul_to_string T1 T2 Tout x y
-               | ident.add T1 T2 Tout
-                 => fun '(x, y)
-                    => add_to_string T1 T2 Tout x y
-               | ident.shiftr T1 Tout offset
-                 => fun v
-                    => (if type.type_beq T1 Tout
-                        then ""
-                        else "(" ++ type.to_string Tout ++ ")")
-                         ++ "(" ++ (*"(" ++ type.to_string T1 ++ ")" ++*) v ++ " >> " ++ Z.to_decimal_string offset ++ ")"
-               | ident.land T1 Tout mask
-                 => fun v
-                    => (if type.type_beq T1 Tout
-                        then ""
-                        else "(" ++ type.to_string Tout ++ ")")
-                         ++ "(" ++ (*"(" ++ type.to_string T1 ++ ")" ++*) v ++ " & " ++ Z.to_hex_string mask ++ primitive.to_UL_postfix Tout ++ ")"
-               | ident.cast T1 Tout
-                 => fun v
-                    => "(" ++ type.to_string Tout ++ ")" ++ v
-               end.
-        End ident.
+      Fixpoint expr_of_PHOAS
+               {t}
+               (e : @Compilers.Uncurried.expr.default.Notations.expr var_data t)
+               (count : positive)
+               (make_name : positive -> option string)
+               {struct e}
+        : forall (ret_val : var_data t), option expr
+        := match e in expr.expr t return var_data t -> option expr with
+           | ((ident.Let_In Compilers.type.Z _)
+                @@ (e1, Abs Compilers.type.Z d e2))%expr
+             => fun v : var_data _
+                => (v <- type.try_transport var_data _ d v;
+                      e1 <- type.try_transport expr.expr _ Compilers.type.Z e1;
+                      e2 <- type.try_transport (fun s => var_data s -> option expr) _ Compilers.type.Z (fun rv => @expr_of_PHOAS d (e2 rv) (Pos.succ count) make_name v);
+                      e1 <- arith_expr_of_PHOAS e1 None;
+                      let '(e1, r1) := e1 in
+                      n1 <- make_name count;
+                        e2 <- e2 (n1, r1);
+                        Some (Seq
+                                (Assign true type.Z r1 n1 e1)
+                                e2))
+           | ((ident.Let_In (Compilers.type.Z * Compilers.type.Z)%ctype _)
+                @@ ((ident.Z_cast2 (r1, r2)%core)
+                      @@ (ident.Z_mul_split_concrete s @@ (x1, x2)),
+                    Abs (Compilers.type.Z * Compilers.type.Z)%ctype d e2))%expr
+             => fun v : var_data _
+                => make_assign_2arg_1ref
+                     (Some r1) (Some r2)
+                     x1 x2 (Z_mul_split s) count make_name v
+                     (fun v rv => @expr_of_PHOAS d (e2 rv) (Pos.succ (Pos.succ count)) make_name v)
+           | ((ident.Let_In (Compilers.type.Z * Compilers.type.Z)%ctype _)
+                @@ (ident.Z_mul_split_concrete s @@ (x1, x2),
+                    Abs (Compilers.type.Z * Compilers.type.Z)%ctype d e2))%expr
+             => fun v : var_data _
+                => make_assign_2arg_1ref
+                     None None
+                     x1 x2 (Z_mul_split s) count make_name v
+                     (fun v rv => @expr_of_PHOAS d (e2 rv) (Pos.succ (Pos.succ count)) make_name v)
+           | ((ident.Let_In (Compilers.type.Z * Compilers.type.Z)%ctype _)
+                @@ ((ident.Z_cast2 (r1, r2)%core)
+                      @@ (ident.Z_add_get_carry_concrete s @@ (x1, x2)),
+                    Abs (Compilers.type.Z * Compilers.type.Z)%ctype d e2))%expr
+             => fun v : var_data _
+                => make_assign_2arg_1ref
+                     (Some r1) (Some r2)
+                     x1 x2 (Z_add_get_carry s) count make_name v
+                     (fun v rv => @expr_of_PHOAS d (e2 rv) (Pos.succ (Pos.succ count)) make_name v)
+           | ((ident.Let_In (Compilers.type.Z * Compilers.type.Z)%ctype _)
+                @@ (ident.Z_add_get_carry_concrete s @@ (x1, x2),
+                    Abs (Compilers.type.Z * Compilers.type.Z)%ctype d e2))%expr
+             => fun v : var_data _
+                => make_assign_2arg_1ref
+                     None None
+                     x1 x2 (Z_add_get_carry s) count make_name v
+                     (fun v rv => @expr_of_PHOAS d (e2 rv) (Pos.succ (Pos.succ count)) make_name v)
+           | ((ident.Let_In (Compilers.type.Z * Compilers.type.Z)%ctype _)
+                @@ ((ident.Z_cast2 (r1, r2)%core)
+                      @@ (ident.Z_sub_get_borrow_concrete s @@ (x1, x2)),
+                    Abs (Compilers.type.Z * Compilers.type.Z)%ctype d e2))%expr
+             => fun v : var_data _
+                => make_assign_2arg_1ref
+                     (Some r1) (Some r2)
+                     x1 x2 (Z_sub_get_borrow s) count make_name v
+                     (fun v rv => @expr_of_PHOAS d (e2 rv) (Pos.succ (Pos.succ count)) make_name v)
+           | ((ident.Let_In (Compilers.type.Z * Compilers.type.Z)%ctype _)
+                @@ (ident.Z_sub_get_borrow_concrete s @@ (x1, x2),
+                    Abs (Compilers.type.Z * Compilers.type.Z)%ctype d e2))%expr
+             => fun v : var_data _
+                => make_assign_2arg_1ref
+                     None None
+                     x1 x2 (Z_sub_get_borrow s) count make_name v
+                     (fun v rv => @expr_of_PHOAS d (e2 rv) (Pos.succ (Pos.succ count)) make_name v)
+           | ((ident.Let_In (Compilers.type.Z * Compilers.type.Z)%ctype _)
+                @@ ((ident.Z_cast2 (r1, r2)%core)
+                      @@ (ident.Z_add_with_get_carry_concrete s @@ (x1, x2, x3)),
+                    Abs (Compilers.type.Z * Compilers.type.Z)%ctype d e2))%expr
+             => fun v : var_data _
+                => make_assign_3arg_1ref
+                     (Some r1) (Some r2)
+                     x1 x2 x3 (Z_add_with_get_carry s) count make_name v
+                     (fun v rv => @expr_of_PHOAS d (e2 rv) (Pos.succ (Pos.succ count)) make_name v)
+           | ((ident.Let_In (Compilers.type.Z * Compilers.type.Z)%ctype _)
+                @@ (ident.Z_add_with_get_carry_concrete s @@ (x1, x2, x3),
+                    Abs (Compilers.type.Z * Compilers.type.Z)%ctype d e2))%expr
+             => fun v : var_data _
+                => make_assign_3arg_1ref
+                     None None
+                     x1 x2 x3 (Z_add_with_get_carry s) count make_name v
+                     (fun v rv => @expr_of_PHOAS d (e2 rv) (Pos.succ (Pos.succ count)) make_name v)
+           | expr.AppIdent s d idc args
+             => fun v : var_data d
+                => (* Coq's deep pattern matching breaks well-typedness, so we kludge around it with transport *)
+                  (args <- type.try_transport expr.expr _ _ args;
+                     make_return_assignment_of_arith v (@expr.AppIdent _ _ s d idc args))
+           | expr.Var _ _ as e
+           | expr.Pair _ _ _ _ as e
+           | expr.TT as e
+           | App _ _ _ _ as e
+           | Abs _ _ _ as e
+             => fun v => make_return_assignment_of_arith v e
+           end%option.
 
-        Module expr.
-          Fixpoint make_assignment (x : string) (t : type) : type.string_interp t -> list string
-            := match t return type.string_interp t -> list string with
-               | type.type_primitive t
-                 => fun body
-                    => [(type.primitive.to_string t ++ " ")
-                          ++ x ++ " = " ++ body ++ ";"]
-               | type.prod A B
-                 => fun '(a, b)
-                    => ((make_assignment (x ++ "₁")%string A a)
-                          ++ (make_assignment (x ++ "₂")%string B b))%list
-               | type.list A
-                 => fun _
-                    => ["#error ""non-return list assignment not supported"";"]
-               end.
+      Fixpoint var_data_of_bounds {t}
+               (count : positive)
+               (make_name : positive -> option string)
+               {struct t}
+        : ZRange.type.option.interp t -> option (positive * var_data t)
+        := match t return ZRange.type.option.interp t -> option (positive * var_data t) with
+           | Compilers.type.Z
+             => fun r => (n <- make_name count;
+                            Some (Pos.succ count, (n, r)))
+           | Compilers.type.prod A B
+             => fun '(ra, rb)
+                => (va <- @var_data_of_bounds A count make_name ra;
+                      let '(count, va) := va in
+                      vb <- @var_data_of_bounds B count make_name rb;
+                        let '(count, vb) := vb in
+                        Some (count, (va, vb)))
+           | type.list Compilers.type.Z
+             => fun r
+                => (ls <- r;
+                      n <- make_name count;
+                      Some (Pos.succ count,
+                            (n,
+                             match ls with
+                             | nil => None
+                             | cons x xs
+                               => List.fold_right
+                                    (fun r1 r2 => r1 <- r1; r2 <- r2; Some (ZRange.union r1 r2))
+                                    x
+                                    xs
+                             end,
+                             List.length ls)))
+           | Compilers.type.unit
+             => fun _ => Some (count, tt)
+           | type.nat
+           | type.bool
+           | type.arrow _ _
+           | type.list _
+             => fun _ => None
+           end%option.
 
-          Fixpoint make_ret_assignment (x : string) (t : type) : type.string_interp t -> list string
-            := match t return type.string_interp t -> list string with
-               | type.type_primitive t
-                 => fun body
-                    => ["*" ++ x ++ " = " ++ body ++ ";"]
-               | type.prod A B
-                 => fun '(a, b)
-                    => ((make_ret_assignment (x ++ "₁")%string A a)
-                          ++ (make_ret_assignment (x ++ "₂")%string B b))%list
-               | type.list A
-                 => fun ls
-                    => match ls with
-                       | inl ls
-                         => map2
-                              (fun n body
-                               => x ++ "[" ++ Z.to_decimal_string (Z.of_nat n) ++ "] = " ++ body ++ ";")%string
-                              (seq 0 (List.length ls))
-                              ls
-                       | inr sls
-                         => [x ++ " = " ++ sls ++ ";"]
-                       end
-               end.
+      Definition ExprOfPHOAS
+               {s d}
+               (e : @Compilers.Uncurried.expr.default.Notations.Expr (s -> d))
+               (name_list : option (list string))
+               (inbounds : ZRange.type.option.interp s)
+        : option (var_data s * var_data d * expr)
+        := (f1 <- invert_Abs (e _);
+              f2 <- invert_Abs (e _);
+              let outbounds := partial.bounds.expr.extract (f1 inbounds) in
+              let make_name := match name_list with
+                               | None => fun p => Some ("x" ++ Z.to_decimal_string (Zpos p))
+                               | Some ls => fun p => List.nth_error ls (pred (Pos.to_nat p))
+                               end in
+              vs <- var_data_of_bounds 1 make_name inbounds;
+                let '(count, vs) := vs in
+                vd <- var_data_of_bounds count make_name outbounds;
+                  let '(count, vd) := vd in
+                  rv <- expr_of_PHOAS (f2 vs) count make_name vd;
+                    Some (vs, vd, rv))%option.
 
-          Fixpoint var_to_string (x : string) (t : type) : type.string_interp t
-            := match t return type.string_interp t with
-               | type.type_primitive t => x
-               | type.prod A B => (var_to_string (x ++ "₁") A,
-                                   var_to_string (x ++ "₂") B)
-               | type.list A => inr x
-               end.
+      Fixpoint arith_to_string {t} (e : arith_expr t) : string
+        := match e with
+           | (literal v @@ _) => primitive.to_string (t:=type.Z) v
+           | (List_nth n @@ Var _ v)
+             => "(" ++ v ++ "[" ++ Z.to_decimal_string (Z.of_nat n) ++ "])"
+           | (Addr @@ Var _ v) => "&" ++ v
+           | (Dereference @@ e) => "( *" ++ @arith_to_string _ e ++ " )"
+           | (Z_shiftr offset @@ e)
+             => "(" ++ @arith_to_string _ e ++ " >> " ++ Z.to_decimal_string offset ++ ")"
+           | (Z_shiftl offset @@ e)
+             => "(" ++ @arith_to_string _ e ++ " << " ++ Z.to_decimal_string offset ++ ")"
+           | (Z_land mask @@ e)
+             => "(" ++ @arith_to_string _ e ++ " & " ++ primitive.to_string (t:=type.Z) mask ++ ")"
+           | (Z_add @@ (x1, x2))
+             => "(" ++ @arith_to_string _ x1 ++ " + " ++ @arith_to_string _ x2 ++ ")"
+           | (Z_mul @@ (x1, x2))
+             => "(" ++ @arith_to_string _ x1 ++ " * " ++ @arith_to_string _ x2 ++ ")"
+           | (Z_sub @@ (x1, x2))
+             => "(" ++ @arith_to_string _ x1 ++ " - " ++ @arith_to_string _ x2 ++ ")"
+           | (Z_opp @@ e)
+             => "(-" ++ @arith_to_string _ e ++ ")"
+           | (Z_mul_split s @@ (x1, x2, x3))
+             => "_mulx_u"
+                  ++ Z.to_decimal_string (Z.log2_up s) ++ "("
+                  ++ @arith_to_string _ x1 ++ ", "
+                  ++ @arith_to_string _ x2 ++ ", "
+                  ++ @arith_to_string _ x3 ++ ")"
+           | (Z_add_get_carry s @@ (x1, x2, x3))
+             => "_add_carryx_u"
+                  ++ Z.to_decimal_string (Z.log2_up s) ++ "(0, "
+                  ++ @arith_to_string _ x1 ++ ", "
+                  ++ @arith_to_string _ x2 ++ ", "
+                  ++ @arith_to_string _ x3 ++ ")"
+           | (Z_add_with_get_carry s @@ (x1, x2, x3, x4))
+             => "_add_carryx_u"
+                  ++ Z.to_decimal_string (Z.log2_up s) ++ "("
+                  ++ @arith_to_string _ x1 ++ ", "
+                  ++ @arith_to_string _ x2 ++ ", "
+                  ++ @arith_to_string _ x3 ++ ", "
+                  ++ @arith_to_string _ x4 ++ ")"
+           | (Z_sub_get_borrow s @@ (x1, x2, x3))
+             => "_subborrow_u"
+                  ++ Z.to_decimal_string (Z.log2_up s) ++ "(0, "
+                  ++ @arith_to_string _ x1 ++ ", "
+                  ++ @arith_to_string _ x2 ++ ", "
+                  ++ @arith_to_string _ x3 ++ ")"
+           | (Z_zselect @@ (cond, et, ef)) => "#error zselect;"
+           | (Z_add_modulo @@ (x1, x2, x3)) => "#error addmodulo;"
+           | (Z_static_cast range @@ e)
+             => "(" ++ String.type.primitive.to_string_relaxed type.Z (Some range) ++ ")"
+                    ++ @arith_to_string _ e
+           | Var _ v => v
+           | (List_nth _ @@ _)
+           | (Addr @@ _)
+           | (Z_add @@ _)
+           | (Z_mul @@ _)
+           | (Z_sub @@ _)
+           | (Z_mul_split _ @@ _)
+           | (Z_add_get_carry _ @@ _)
+           | (Z_add_with_get_carry _ @@ _)
+           | (Z_sub_get_borrow _ @@ _)
+           | (Z_zselect @@ _)
+           | (Z_add_modulo @@ _)
+             => "#error bad_arg;"
+           | Pair A B a b
+             => "#error pair;"
+           | TT
+             => "#error tt;"
+           end%core%Cexpr.
 
-          Fixpoint to_string' (x : string) {t} (e : @expr ident t)
-            : (type.string_interp t -> list string) -> list string
-            := match e in expr.expr t return (type.string_interp t -> _) -> _ with
-               | expr.Var t p
-                 => fun k
-                    => k (var_to_string (x ++ decimal_string_of_pos p) t)
-               | expr.TT => fun k => k "()"
-               | expr.AppIdent s d idc args
-                 => fun k
-                    => @to_string'
-                         x s args
-                         (fun v
-                          => k (ident.to_string idc v))
-               | expr.Pair A B a b
-                 => fun k =>
-                      @to_string'
-                        x A a
-                        (fun a => @to_string'
-                                    x B b
-                                    (fun b => k (a, b)))
-               | expr.Let_In s d n ex body
-                 => fun k
-                    => @to_string'
-                         x s ex
-                         (fun xv
-                          => (make_assignment
-                                (x ++ decimal_string_of_pos n)
-                                s
-                                xv)
-                               ++ @to_string' x d body k)%list
-               end.
+      Fixpoint to_strings (e : expr) : list string
+        := match e with
+           | Seq e1 e2 => (to_strings e1 ++ to_strings e2)%list
+           | Assign true t sz name val
+             => [String.type.primitive.to_string_relaxed t sz ++ " " ++ name ++ " = " ++ arith_to_string val ++ ";"]
+           | Assign false _ sz name val
+             => [name ++ " = " ++ arith_to_string val ++ ";"]
+           | AssignZPtr name sz val
+             => ["*" ++ name ++ " = " ++ arith_to_string val ++ ";"]
+           | DeclareVar t sz name
+             => [String.type.primitive.to_string_relaxed t sz ++ " " ++ name ++ ";"]
+           | AssignNth name n val
+             => [name ++ "[" ++ Z.to_decimal_string (Z.of_nat n) ++ "] = " ++ arith_to_string val ++ ";" ]
+           end.
 
-          Local Notation NewLine := (String "010" "") (only parsing).
+      Fixpoint to_arg_list {t} : var_data t -> list string
+        := match t return var_data t -> _ with
+           | Compilers.type.Z
+             => fun '(n, r) => [String.type.primitive.to_string_relaxed type.Z r ++ " " ++ n]
+           | Compilers.type.prod A B
+             => fun '(va, vb) => (@to_arg_list A va ++ @to_arg_list B vb)%list
+           | type.list Compilers.type.Z
+             => fun '(n, r, len) => [String.type.primitive.to_string_relaxed type.Z r ++ "[" ++ Z.to_decimal_string (Z.of_nat len) ++ "] " ++ n]
+           | type.list _ => fun _ => ["#error ""complex list"";"]
+           | Compilers.type.unit => fun _ => ["#error unit;"]
+           | type.nat => fun _ => ["#error ℕ;"]
+           | type.bool => fun _ => ["#error bool;"]
+           | type.arrow _ _ => fun _ => ["#error arrow;"]
+           end.
 
-          Local Notation var_prefix := "x".
-          Local Notation ret_prefix := "ret".
+      Fixpoint to_retarg_list {t} : var_data t -> list string
+        := match t return var_data t -> _ with
+           | Compilers.type.Z
+             => fun '(n, r) => [String.type.primitive.to_string_relaxed type.Zptr r ++ " " ++ n]
+           | Compilers.type.prod A B
+             => fun '(va, vb) => (@to_retarg_list A va ++ @to_retarg_list B vb)%list
+           | type.list Compilers.type.Z
+             => fun '(n, r, len) => [String.type.primitive.to_string_relaxed type.Z r ++ "[" ++ Z.to_decimal_string (Z.of_nat len) ++ "] " ++ n]
+           | type.list _ => fun _ => ["#error ""complex list"";"]
+           | Compilers.type.unit => fun _ => ["#error unit;"]
+           | type.nat => fun _ => ["#error ℕ;"]
+           | type.bool => fun _ => ["#error bool;"]
+           | type.arrow _ _ => fun _ => ["#error arrow;"]
+           end.
 
-          Definition to_lines (indent : string) {t} (e : @expr ident t)
-            : list string
-            := List.map (fun v => indent ++ v)
-                        (to_string'
-                           var_prefix e
-                           (fun retval
-                            => make_ret_assignment ret_prefix _ retval)).
+      Fixpoint join (sep : string) (ls : list string) : string
+        := match ls with
+           | nil => ""
+           | cons x nil => x
+           | cons x xs => x ++ sep ++ join sep xs
+           end.
 
-          Definition to_string (indent : string) {t} (e : @expr ident t)
-            : string
-            := List.fold_right
-                 (fun a b => a ++ NewLine ++ b)
-                 ""
-                 (to_lines indent e).
+      Definition to_function_lines (name : string)
+                 {s d}
+                 (f : var_data s * var_data d * expr)
+        : list string
+        := let '(args, rets, body) := f in
+           (((("void "
+                 ++ name ++ "("
+                 ++ (join ", " (to_arg_list args ++ to_retarg_list rets))
+                 ++ ") {")%string)
+               :: (List.map (fun s => "  " ++ s)%string (to_strings body)))
+              ++ ["}"])%list.
 
-          Fixpoint make_arg_list (by_ref : bool)
-                   {t}
-            : type.string_interp t -> list string
-            := match t return type.string_interp t -> list string with
-               | type.type_primitive t
-                 => fun n => [(type.primitive.to_string t) ++ " " ++ (if by_ref then "*" else "") ++ n]
-               | type.prod A B
-                 => fun '(a, b) => (@make_arg_list by_ref A a ++ @make_arg_list by_ref B b)%list
-               | type.list A
-                 => fun ls
-                    => [(type.primitive.to_string A ++ " *")
-                          ++ match ls with
-                             | inl ls
-                               => List.hd "" ls
-                             | inr sls
-                               => sls
-                             end]
-               end.
+      Local Notation NewLine := (String "010" "") (only parsing).
 
-          Fixpoint join (sep : string) (ls : list string) : string
-            := match ls with
-               | nil => ""
-               | cons x nil => x
-               | cons x xs => x ++ sep ++ join sep xs
-               end.
+      Definition ToFunctionLines (name : string)
+                 {s d}
+                 (e : @Compilers.Uncurried.expr.default.Notations.Expr (s -> d))
+                 (name_list : option (list string))
+                 (inbounds : ZRange.type.option.interp s)
+        : option (list string)
+        := (f <- ExprOfPHOAS e name_list inbounds;
+              Some (to_function_lines name f)).
 
-          Definition to_function_lines (name : string)
-                     (argT : type)
-                     {t} (e : @expr ident t)
-            : list string
-            := (("void "
-                   ++ name ++ "("
-                   ++ (join
-                         ", "
-                         ((make_arg_list false (var_to_string var_prefix argT) )
-                            ++ make_arg_list true (var_to_string ret_prefix t)))
-                   ++ ") {")
-                  :: ((to_lines "  " e)
-                        ++ ["}"])%list).
-
-          Definition to_function_string (name : string)
-                     (argT : type)
-                     {t} (e : @expr ident t)
-            : string
-            := join NewLine (to_function_lines name argT e).
-        End expr.
-      End ToString.
-    End Indexed.
-    Module Export Notations.
-      Export BoundsAnalysis.type.Notations.
-      Export BoundsAnalysis.Indexed.expr.Notations.
-      Export BoundsAnalysis.ident.Notations.
-      Import BoundsAnalysis.type.
-      Import BoundsAnalysis.Indexed.expr.
-      Import BoundsAnalysis.ident.
-      Notation "[ ]" := (AppIdent ident.nil _) : nexpr_scope.
-      Notation "x :: xs" := (AppIdent ident.cons (Pair x%nexpr xs%nexpr)) : nexpr_scope.
-      Notation "x" := (AppIdent (ident.primitive x) _) (only printing, at level 9) : nexpr_scope.
-      Notation "ls [[ n ]]"
-        := (AppIdent ident.List.nth_default (_, ls, AppIdent (ident.primitive n%nat) _)%nexpr)
-           : nexpr_scope.
-      Notation "'x_' n" := (Var _ n) (at level 10, format "'x_' n") : nexpr_scope.
-    End Notations.
-
-    Module AdjustBounds.
-      Local Notation "( a ; b )" := (existT _ a b) : core_scope.
-      Import Indexed.
-      Import type expr ident.
-      Module ident.
-        Section with_relax.
-          Context (relax_zrange : zrange -> option zrange).
-
-          Local Notation primitive_for_zrange := (primitive_for_zrange relax_zrange).
-
-          Fixpoint type_for_range {t} : range t -> type
-            := match t return range t -> type with
-               | type_primitive _ => primitive_for_zrange
-               | prod A B => fun (ab : range A * range B)
-                             => prod (@type_for_range A (Datatypes.fst ab))
-                                     (@type_for_range B (Datatypes.snd ab))
-               | list A
-                 => fun ls : Datatypes.list zrange
-                    => type.list
-                         (primitive_for_zrange (List.fold_right ZRange.union r[0 ~> 0]%zrange ls))
-               end.
-
-          Definition upper_lor_and_bounds (x y : BinInt.Z) : BinInt.Z
-            := 2^(1 + Z.log2_up (Z.max x y)).
-          Definition extreme_lor_land_bounds (x y : zrange) : zrange
-            := let mx := ZRange.upper (ZRange.abs x) in
-               let my := ZRange.upper (ZRange.abs y) in
-               {| lower := -upper_lor_and_bounds mx my ; upper := upper_lor_and_bounds mx my |}.
-          Definition extremization_bounds (f : zrange -> zrange -> zrange) (x y : zrange) : zrange
-            := let (lx, ux) := x in
-               let (ly, uy) := y in
-               if ((lx <? 0) || (ly <? 0))%Z%bool
-               then extreme_lor_land_bounds x y
-               else f x y.
-          Definition land_bounds : zrange -> zrange -> zrange
-            := extremization_bounds
-                 (fun x y
-                  => let (lx, ux) := x in
-                     let (ly, uy) := y in
-                     {| lower := Z.min 0 (Z.min lx ly) ; upper := Z.max 0 (Z.min ux uy) |}).
-
-          (** TODO: Move me *)
-          Definition smart_fst {A B} (e : @expr ident (A * B)) : @expr ident A
-            := match e in @expr _ t
-                     return @expr ident match t with
-                                        | type.prod A B => A
-                                        | _ => A
-                                        end
-                            -> @expr ident match t with
-                                           | type.prod A B => A
-                                           | _ => A
-                                           end
-               with
-               | Pair A B a b => fun _ => a
-               | _ => fun x => x
-               end (AppIdent fst e).
-          Definition smart_snd {A B} (e : @expr ident (A * B)) : @expr ident B
-            := match e in @expr _ t
-                     return @expr ident match t with
-                                        | type.prod A B => B
-                                        | _ => B
-                                        end
-                            -> @expr ident match t with
-                                           | type.prod A B => B
-                                           | _ => B
-                                           end
-               with
-               | Pair A B a b => fun _ => b
-               | _ => fun x => x
-               end (AppIdent snd e).
-          Definition smart_cast {A B : type.primitive} (e : @expr ident A) : @expr ident B
-            := match transport (@expr ident) A B e with
-               | Some e' => e'
-               | None => AppIdent (cast A B) e
-               end.
-
-          (** We would like to just write the following.  Alas, we must await a solution to COQBUG(https://github.com/coq/coq/issues/6320) *)
-          (**
-<<
-          Fixpoint list_map {A B : type.primitive}
-                   (f : @expr ident A -> @expr ident B)
-                   (e : @expr ident (type.list A))
-            : option (@expr ident (type.list B))
-            := match e with
-               | AppIdent _ _ (ident.nil _) _
-                 => Some (AppIdent ident.nil TT)
-               | AppIdent _ _ (ident.cons _) (Pair _ _ x xs)
-                 => option_map
-                      (fun f_xs => AppIdent ident.cons (f x, f_xs))
-                      (@list_map _ _ f xs)
-               | _ => None
-               end.
->> *)
-          Fixpoint list_map {A B : type.primitive}
-                   (f : @expr ident A -> @expr ident B)
-                   (e : @expr ident (type.list A))
-            : option (@expr ident (type.list B))
-            := match e in @expr _ T
-                     return (@expr ident match T with
-                                         | type.list A => A
-                                         | _ => A
-                                         end
-                             -> @expr ident B)
-                            -> option (@expr ident (type.list B))
-               with
-               | AppIdent s (type.list d) idc args
-                 => match args in expr s
-                          return ident s (type.list d)
-                                 -> (@expr ident d -> @expr ident B)
-                                 -> option (expr (type.list B))
-                    with
-                    | Pair A' (type.list B') a' b'
-                      => fun idc f
-                         => match idc in ident s d
-                                  return (match s return Type with
-                                          | type.prod A _ => expr A
-                                          | _ => Datatypes.unit
-                                          end
-                                          -> match s return Type with
-                                             | type.prod _ (type.list A)
-                                               => (expr A -> expr B)
-                                                  -> option (expr (type.list B))
-                                             | _ => Datatypes.unit
-                                             end
-                                          -> match d return Type with
-                                             | type.list d
-                                               => expr d -> expr B
-                                             | _ => Datatypes.unit
-                                             end
-                                          -> option (expr (type.list B)))
-                            with
-                            | ident.nil t
-                              => fun _ _ _ => Some (AppIdent ident.nil TT)
-                            | ident.cons t
-                              => fun x rec_xs f
-                                 => option_map
-                                      (fun f_xs => AppIdent ident.cons (f x, f_xs))
-                                      (rec_xs f)
-                            | _ => fun _ _ _ => None
-                            end a' (fun f => @list_map _ _ f b') f
-                    | TT
-                      => match idc with
-                         | ident.nil _
-                           => fun _ _ => Some (AppIdent ident.nil TT)
-                         | _ => fun _ _ => None
-                         end
-                    | _ => fun _ _ => None
-                    end idc
-               | _ => fun _ => None
-               end f.
-
-          Definition adjust_bounds {s d} (idc : ident s d)
-            : option { r : range s & @expr ident (type_for_range r) }
-              -> option { r : range d & @expr ident (type_for_range r) }
-            := match idc in ident s d
-                     return option { r : range s & @expr ident (type_for_range r) }
-                            -> option { r : range d & @expr ident (type_for_range r) }
-               with
-               | primitive type.Z v
-               | primitive (type.ZBounded _ _) v
-                 => fun _ => Some (existT
-                                     (fun r : range type.Z => @expr ident (type_for_range r))
-                                     r[v~>v]%zrange
-                                     (AppIdent (primitive (t:=primitive_for_zrange r[v~>v])
-                                                          match relax_zrange r[v ~> v] as t
-                                                                return type.interp (primitive_for_option_zrange t)
-                                                          with
-                                                          | Some _ => {| value := v ; value_bounded := admit (* XXX needs proof about relax *) |}
-                                                          | None => v
-                                                          end)
-                                               TT))
-               | primitive type.unit _ as idc
-                 => fun _ => None
-               | nil _ as idc
-                 => fun _ => Some (existT _ Datatypes.nil (AppIdent nil TT))
-               | cons t
-                 => fun args
-                    => args' <- args;
-                         let '(r; args) := args' in
-                         snd_args <- (list_map
-                                        smart_cast
-                                        (smart_snd args));
-                           Some ((Datatypes.fst r :: Datatypes.snd r);
-                                   (AppIdent
-                                      cons
-                                      (smart_cast (smart_fst args),
-                                       snd_args)))
-               | fst A B
-                 => option_map
-                      (fun '(existT r args)
-                       => existT _ (Datatypes.fst r) (AppIdent fst args))
-               | snd A B
-                 => option_map
-                      (fun '(existT r args)
-                       => existT _ (Datatypes.snd r) (AppIdent snd args))
-               | List_nth T n
-                 => option_map
-                      (fun '(existT r args)
-		       => existT _ _ (AppIdent (List_nth n) args))
-               | mul _ _ _
-                 => option_map
-                      (fun '(existT r args)
-		       => existT _ (ZRange.four_corners BinInt.Z.mul (Datatypes.fst r) (Datatypes.snd r))
-                                 (AppIdent (mul _ _ _) args))
-               | add _ _ _
-                 => option_map
-                      (fun '(existT r args)
-		       => existT _ (ZRange.four_corners BinInt.Z.add (Datatypes.fst r) (Datatypes.snd r))
-                                 (AppIdent (add _ _ _) args))
-               | shiftr _ _ offset
-                 => option_map
-                      (fun '(existT r args)
-		       => existT _ (ZRange.two_corners (fun v => BinInt.Z.shiftr v offset) r)
-                                 (AppIdent (shiftr _ _ offset) args))
-               | land _ _ mask
-                 => option_map
-                      (fun '(existT r args)
-		       => existT _ (land_bounds r r[mask~>mask]%zrange)
-                                 (AppIdent (land _ _ mask) args))
-               | cast _ (type.ZBounded l u)
-                 => option_map
-                      (fun '(existT r[l'~>u'] args)
-		       => existT _ r[Z.max l l' ~> Z.min u u']
-                                 (AppIdent (cast _ _) args))
-               | cast _ _
-                 => fun _ => None
-               end%zrange%option.
-        End with_relax.
-      End ident.
->>>>>>> Write a C string generator for synthesized code
+      Definition ToFunctionString (name : string)
+                 {s d}
+                 (e : @Compilers.Uncurried.expr.default.Notations.Expr (s -> d))
+                 (name_list : option (list string))
+                 (inbounds : ZRange.type.option.interp s)
+        : option string
+        := (ls <- ToFunctionLines name e name_list inbounds;
+              Some (join NewLine ls)).
+    End C.
+    Notation ToFunctionLines := C.ToFunctionLines.
+    Notation ToFunctionString := C.ToFunctionString.
+  End ToString.
 End Compilers.
 Import Associational Positional Compilers.
 Local Coercion Z.of_nat : nat >-> Z.
@@ -7314,7 +7712,7 @@ Section rcarry_mul.
          (fun v : Z => Qceiling (11/10 * v))
          (encode (weight (Qnum limbwidth) (Qden limbwidth)) n s c (s-1)).
   Let default_upperbound_tight := (2^Qceiling limbwidth + 2^(Qceiling limbwidth - 3))%Z.
-  Let prime_bound : ZRange.type.option.interp (type.Z)
+  Definition prime_bound : ZRange.type.option.interp (type.Z)
     := Some r[0~>(s - Associational.eval c - 1)]%zrange.
 
   Definition relax_zrange_of_machine_wordsize
@@ -7328,9 +7726,9 @@ Section rcarry_mul.
          (seq 0 len).
   Let tight_upperbounds : list Z
     := adjust_list_to_length default_upperbound_tight precise_tight_upperbounds n.
-  Let tight_bounds : list (ZRange.type.option.interp type.Z)
+  Definition tight_bounds : list (ZRange.type.option.interp type.Z)
     := List.map (fun u => Some r[0~>u]%zrange) tight_upperbounds.
-  Let loose_bounds : list (ZRange.type.option.interp type.Z)
+  Definition loose_bounds : list (ZRange.type.option.interp type.Z)
     := List.map (fun u => Some r[0 ~> 3*u]%zrange) tight_upperbounds.
 
   Definition check_args {T} (res : Pipeline.ErrorT T)
@@ -7491,6 +7889,7 @@ Section rcarry_mul.
     Proof.
       clear -curve_good.
       cbv [check_args] in curve_good.
+      cbv [tight_bounds loose_bounds prime_bound] in *.
       break_innermost_match_hyps; try discriminate.
       rewrite negb_false_iff in *.
       Z.ltb_to_lt.
@@ -7850,11 +8249,9 @@ Module X25519_64.
   Definition s := 2^255.
   Definition c := [(1, 19)].
   Definition machine_wordsize := 64.
-<<<<<<< d97e060a3f8de0b83db89aa6c25eb4157045c275
-||||||| merged common ancestors
-=======
-  Definition arg_type := (BoundsAnalysis.AdjustBounds.ident.type_for_range relax_zrange (t:=BoundsAnalysis.Indexed.OfPHOAS.type.compile (type.list type.Z * type.list type.Z)) (f_bounds, f_bounds)).
->>>>>>> Write a C string generator for synthesized code
+  Local Notation tight_bounds := (tight_bounds n s c).
+  Local Notation loose_bounds := (loose_bounds n s c).
+  Local Notation prime_bound := (prime_bound s c).
 
   Derive base_51_relax
          SuchThat (rrelax_correctT n s c machine_wordsize base_51_relax)
@@ -7977,38 +8374,24 @@ fun var : type -> Type =>
              type.list (type.type_primitive type.Z) ->
              type.list (type.type_primitive type.Z)))
 *)
-  Compute BoundsAnalysis.Indexed.ToString.expr.to_function_string
-          "femul"
-          arg_type
-          base_51_carry_mul.
+
+  Compute ToString.C.ToFunctionString
+          "fecarry_mul" base_51_carry_mul
+          None (Some loose_bounds, Some loose_bounds).
   (*
-void femul(uint64_t *x₁, uint64_t *x₂, uint64_t *ret) {
-  uint128_t x2 = (((uint128_t)x1₁[0] * x1₂[0]) + ((0x13UL * ((uint128_t)x1₁[1] * x1₂[4])) + ((0x13UL * ((uint128_t)x1₁[2] * x1₂[3])) + ((0x13UL * ((uint128_t)x1₁[3] * x1₂[2])) + (0x13UL * ((uint128_t)x1₁[4] * x1₂[1]))))));
-  uint64_t x3 = (uint64_t)(x2 >> 51);
-  uint64_t x4 = (uint64_t)(x2 & 0x7ffffffffffffUL);
-  uint128_t x5 = (x3 + (((uint128_t)x1₁[0] * x1₂[1]) + (((uint128_t)x1₁[1] * x1₂[0]) + ((0x13UL * ((uint128_t)x1₁[2] * x1₂[4])) + ((0x13UL * ((uint128_t)x1₁[3] * x1₂[3])) + (0x13UL * ((uint128_t)x1₁[4] * x1₂[2])))))));
-  uint64_t x6 = (uint64_t)(x5 >> 51);
-  uint64_t x7 = (uint64_t)(x5 & 0x7ffffffffffffUL);
-  uint128_t x8 = (x6 + (((uint128_t)x1₁[0] * x1₂[2]) + (((uint128_t)x1₁[1] * x1₂[1]) + (((uint128_t)x1₁[2] * x1₂[0]) + ((0x13UL * ((uint128_t)x1₁[3] * x1₂[4])) + (0x13UL * ((uint128_t)x1₁[4] * x1₂[3])))))));
-  uint64_t x9 = (uint64_t)(x8 >> 51);
-  uint64_t x10 = (uint64_t)(x8 & 0x7ffffffffffffUL);
-  uint128_t x11 = (x9 + (((uint128_t)x1₁[0] * x1₂[3]) + (((uint128_t)x1₁[1] * x1₂[2]) + (((uint128_t)x1₁[2] * x1₂[1]) + (((uint128_t)x1₁[3] * x1₂[0]) + (0x13UL * ((uint128_t)x1₁[4] * x1₂[4])))))));
-  uint64_t x12 = (uint64_t)(x11 >> 51);
-  uint64_t x13 = (uint64_t)(x11 & 0x7ffffffffffffUL);
-  uint128_t x14 = (x12 + (((uint128_t)x1₁[0] * x1₂[4]) + (((uint128_t)x1₁[1] * x1₂[3]) + (((uint128_t)x1₁[2] * x1₂[2]) + (((uint128_t)x1₁[3] * x1₂[1]) + ((uint128_t)x1₁[4] * x1₂[0]))))));
-  uint64_t x15 = (uint64_t)(x14 >> 51);
-  uint64_t x16 = (uint64_t)(x14 & 0x7ffffffffffffUL);
-  uint64_t x17 = (x4 + (0x13UL * x15));
-  uint64_t x18 = (x17 >> 51);
-  uint64_t x19 = (x17 & 0x7ffffffffffffUL);
-  uint64_t x20 = (x18 + x7);
-  uint64_t x21 = (x20 >> 51);
-  uint64_t x22 = (x20 & 0x7ffffffffffffUL);
-  ret[0] = x19;
-  ret[1] = x22;
-  ret[2] = (x21 + x10);
-  ret[3] = x13;
-  ret[4] = x16;
+void fecarry_mul(uint64_t[5] x1, uint64_t[5] x2, uint64_t[5] x3) {
+  uint64_t x4 = ((uint128_t)((uint128_t)(x1[0]) * (x2[0])) + ((uint128_t)((uint128_t)(x1[1]) * (0x13 * (x2[4]))) + ((uint128_t)((uint128_t)(x1[2]) * (0x13 * (x2[3]))) + ((uint128_t)((uint128_t)(x1[3]) * (0x13 * (x2[2]))) + ((uint128_t)(x1[4]) * (0x13 * (x2[1])))))));
+  uint64_t x5 = ((uint128_t)(x4 >> 51) + ((uint128_t)((uint128_t)(x1[0]) * (x2[1])) + ((uint128_t)((uint128_t)(x1[1]) * (x2[0])) + ((uint128_t)((uint128_t)(x1[2]) * (0x13 * (x2[4]))) + ((uint128_t)((uint128_t)(x1[3]) * (0x13 * (x2[3]))) + ((uint128_t)(x1[4]) * (0x13 * (x2[2]))))))));
+  uint64_t x6 = ((uint128_t)(x5 >> 51) + ((uint128_t)((uint128_t)(x1[0]) * (x2[2])) + ((uint128_t)((uint128_t)(x1[1]) * (x2[1])) + ((uint128_t)((uint128_t)(x1[2]) * (x2[0])) + ((uint128_t)((uint128_t)(x1[3]) * (0x13 * (x2[4]))) + ((uint128_t)(x1[4]) * (0x13 * (x2[3]))))))));
+  uint64_t x7 = ((uint128_t)(x6 >> 51) + ((uint128_t)((uint128_t)(x1[0]) * (x2[3])) + ((uint128_t)((uint128_t)(x1[1]) * (x2[2])) + ((uint128_t)((uint128_t)(x1[2]) * (x2[1])) + ((uint128_t)((uint128_t)(x1[3]) * (x2[0])) + ((uint128_t)(x1[4]) * (0x13 * (x2[4]))))))));
+  uint64_t x8 = ((uint128_t)(x7 >> 51) + ((uint128_t)((uint128_t)(x1[0]) * (x2[4])) + ((uint128_t)((uint128_t)(x1[1]) * (x2[3])) + ((uint128_t)((uint128_t)(x1[2]) * (x2[2])) + ((uint128_t)((uint128_t)(x1[3]) * (x2[1])) + ((uint128_t)(x1[4]) * (x2[0])))))));
+  uint64_t x9 = ((uint64_t)(x4 & 0x7ffffffffffffUL) + (0x13 * (uint64_t)(x8 >> 51)));
+  uint64_t x10 = ((uint64_t)(x9 >> 51) + (x5 & 0x7ffffffffffffUL));
+  x3[0] = (x9 & 0x7ffffffffffffUL);
+  x3[1] = (x10 & 0x7ffffffffffffUL);
+  x3[2] = ((uint64_t)(x10 >> 51) + (x6 & 0x7ffffffffffffUL));
+  x3[3] = (x7 & 0x7ffffffffffffUL);
+  x3[4] = (x8 & 0x7ffffffffffffUL);
 }
 *)
 End X25519_64.
